theories/examples/rand.v
@@ -22,8 +22,7 @@ Section proof.
     dwp_bind (ref #true)%E (ref #true)%E.
     pose (Φ1 := (λ v, ∃ (l : loc), ⌜v = #l⌝ ∗ l ↦ₗ #true)%I).
     pose (Φ2 := (λ v, ∃ (l : loc), ⌜v = #l⌝ ∗ l ↦ᵣ #true)%I).
-    iApply (dwp_atomic_lift_wp_simple Φ1 Φ2%I); try done.
-    repeat iSplitR.
+    iApply (dwp_atomic_lift_wp Φ1 Φ2).
     { rewrite /WP1 /Φ1. wp_alloc l1 as "Hl". eauto with iFrame. }
     { rewrite /WP2 /Φ2. wp_alloc l1 as "Hl". eauto with iFrame. }
     iIntros (? ?).
@@ -43,8 +42,7 @@ Section proof.
       pose (Φ2 := (λ v, ⌜v = #()⌝ ∗ l2 ↦ᵣ #false)%I).
       iApply dwp_atomic.
       iInv N as (b) "[Hl1 Hl2]" "Hcl". iModIntro.
-      iApply (dwp_atomic_lift_wp_simple Φ1 Φ2%I); try done.
-      iSplitL "Hl1"; [|iSplitL "Hl2"].
+      iApply (dwp_atomic_lift_wp Φ1 Φ2 with "[Hl1] [Hl2] [-]"); try done.
       - rewrite /WP1 /Φ1. wp_store. eauto.
       - rewrite /WP2 /Φ2. wp_store. eauto.
       - iIntros (? ?) "[-> Hl1] [-> Hl2]". iNext.
